\documentclass[a4paper,11pt]{article}
\usepackage[T1]{fontenc}
\usepackage[utf8]{inputenc}
\usepackage{lmodern}
\usepackage{ngerman}
\usepackage{amsmath}
\usepackage{amssymb}
\usepackage{amstext}
\usepackage{amsfonts}
\usepackage{mathrsfs}
\usepackage{ragged2e}

\title{}
\author{}

\begin{document}

\begin{flushleft}
\textbf{exercise 3.2 Backpropagation} \\
(a)  
\end{flushleft}

\begin{equation*}
\begin{aligned}
    E(w) &= \frac{1}{L} \sum_{l=1}^L || d_l - f(x_l;w) ||^2_2 \\
    \nabla E(w) &= \frac{2}{L} \sum_{l=1}^L (f(x_l;w) - d_l) \\
    \frac{\partial f}{\partial w_{1,1}^{2,0}} &= \sum_{j=0}^2 w_{0,j}^{1,1} \, x_j \\ 
    \frac{\partial E}{\partial w_{1,1}^{2,0}} &= \frac{2}{L} \sum_{l=1}^L (f(x_l;w) - d_l)  \sum_{j=0}^2 w_{0,j}^{1,1} \, x_j \\
\end{aligned}
\end{equation*}

\begin{flushleft}
(b)
\end{flushleft}

\begin{equation*}
\begin{aligned}
    g(x;w) &= \sum_{j=0}^2 w_{0,j}^{1,1} \, x_j \\
    \frac{\partial g}{\partial w_{0,1}^{1,1}} &= x_1 \\
    \frac{\partial E}{\partial w_{0,1}^{1,1}} &= \frac{2}{L} \sum_{l=1}^L (f(x_l;w) - d_l) \, w_{1,1}^{2,0} \, x_1 
\end{aligned}
\end{equation*}


\end{document}
